TwoMessageP: added more comments

examples/TwoMessageP/DY.TwoMessage.Protocol.fst
@@ -30,6 +30,7 @@ type ack = {
 /// the overall abstract message type
 /// (consisting of constructors for the two messages
 /// and using the above abstract types for each of them)
+
 [@@ with_bytes bytes] // ignore this line for now
 type message =
   | Ping: (msg:ping_t) -> message
@@ -44,8 +45,11 @@ type message =
 /// We are not going into the details of how Comparse works.
 
 
-/// We let Comparse generate a parser `ps_ping` for the abstract `ping` type
+/// We let Comparse generate a parser `ps_ping_t` for the abstract `ping_t` type
+
 %splice [ps_ping_t] (gen_parser (`ping_t))
+
+/// ... and the same for the other abstract message types
 
 %splice [ps_ack] (gen_parser (`ack))
 
@@ -57,6 +61,7 @@ type message =
 /// but this is the step that enables us to call
 /// `parse message buff` and `serialize message msg`
 /// to translate between bytes and our abstract message type.
+
 instance parseable_serializeable_bytes_message: parseable_serializeable bytes message = mk_parseable_serializeable ps_message
 
 
@@ -90,7 +95,7 @@ type state =
   | ReceivedAck: received_ack -> state
 
 /// As for messages, we use Comparse to generate
-/// a parser and serializer for our abstract state type.
+/// a parser and serializer for our abstract state types.
 
 %splice [ps_sent_ping] (gen_parser (`sent_ping))
 %splice [ps_sent_ack] (gen_parser (`sent_ack))
@@ -100,9 +105,11 @@ type state =
 /// Now, we can call
 /// `parse state buff` and `serialize state st`
 /// to translate between bytes and the abstract state type.
+
 instance parseable_serializeable_bytes_state: parseable_serializeable bytes state = mk_parseable_serializeable ps_state
 
-(** TODO **)
+/// We tag our protocol level states,
+/// so that they are distinguishable from any internal DY* states. 
 
 instance local_state_state: local_state state = {
   tag = "P.State";
@@ -111,73 +118,108 @@ instance local_state_state: local_state state = {
 
 (*** The Protocol ***)
 
+/// Alice sends the first message to Bob:
+/// * Alice generates a new nonce [n_a]
+/// * sends the message (Alice, n_a) (intended for Bob)
+/// * stores n_a and Bob in a state (in a new session)
+/// The step returns the ID of the new state
+/// and the timestamp of the message on the trace
+
 val send_ping: principal -> principal -> traceful (state_id & timestamp)
 let send_ping alice bob =
-  // TODO: use public/secret for this label? 
-  // or already explain high-level idea of "intended readers"?
-  let* n_a = mk_rand NoUsage (join (principal_label alice) (principal_label bob)) 32 in
+  // generate a new nonce
+  let* n_a = gen_rand in
+
+  // the abstract message (alice, n_a)
   let ping = Ping {p_alice = alice; p_n_a = n_a} in 
+  // send the message (serialize abstract to bytes first)
   let* msg_ts = send_msg (serialize message ping) in
-  let* sid = start_new_session alice (SentPing {sp_bob = bob; sp_n_a = n_a}) in
+
+  // the abstract new state (bob, n_a)
+  let ping_state = SentPing {sp_bob = bob; sp_n_a = n_a} in
+  // start a new session with this new state
+  let* sid = start_new_session alice ping_state in
+
+  // return the ID of the new session and the timestamp of the message
   return (sid, msg_ts)
 
 
-val decode_ping : bytes -> option ping_t
-let decode_ping msg =
-  let? png = parse message msg in
-  guard (Ping? png);?
-  assert(Ping? png);
-  Some (Ping?.msg png)
+/// Bob receives the first messages and replies:
+/// * read the message (Alice, n_a) from the trace
+/// * send the reply (n_a) (intended for Alice)
+/// * store n_a and Alice in a state in a new session
+/// The step returns the ID of the new state
+/// and the timestamp of the reply on the trace.
+/// The step fails, if
+/// the message is not of the right type, i.e., not a first message.
 
-val receive_ping_and_send_ack: principal -> timestamp -> traceful (option state_id)
+val receive_ping_and_send_ack: principal -> timestamp -> traceful (option (state_id & timestamp))
 let receive_ping_and_send_ack bob msg_ts =
-  let*? msg = recv_msg msg_ts in
-  let*? png = return (decode_ping msg) in
-  let* sess_id = new_session_id bob in
-  set_state bob sess_id (SentAck {sa_alice = png.p_alice; sa_n_a = png.p_n_a});*
-  return (Some sess_id)
-
-
-val receive_ping_and_send_ack_: principal -> timestamp -> traceful (option state_id)
-let receive_ping_and_send_ack_ bob msg_ts =
-  let*? msg = recv_msg msg_ts in
-  match*? return (parse message msg) with
-  | Ping png -> (
-      let* sess_id = new_session_id bob in
-      set_state bob sess_id (SentAck {sa_alice = png.p_alice; sa_n_a = png.p_n_a});*
-      return (Some sess_id)
-  )
-  | _ -> return None
-
-
-
-val receive_ping_and_send_ack___: principal -> timestamp -> traceful (option (state_id & timestamp))
-let receive_ping_and_send_ack___ bob msg_ts =
-  let*? msg = recv_msg msg_ts in
+  // receive the message
+  let*? msg = recv_msg msg_ts in 
+  // this returns bytes, so we need to translate to our abstract type:
   let*? png_ = return (parse message msg) in
+  // check that the received message is of the right type
+  // (the whole step fails, if the message is not a Ping)
   guard_tr (Ping? png_);*?
+
+  // read the data (alice and n_a) from the received message
   let Ping png = png_ in
+  let alice = png.p_alice in
   let n_a = png.p_n_a in
+
+  // the reply (n_a)
   let ack = Ack {a_n_a = n_a} in
+  // send the reply (serialize abstract to bytes first)
   let* ack_ts = send_msg (serialize message ack) in
-  let* sess_id = new_session_id bob in
-  set_state bob sess_id (SentAck {sa_alice = png.p_alice; sa_n_a = png.p_n_a});*
+
+  // the abstract new state storing alice and n_a from the message
+  let ack_state = SentAck {sa_alice = alice; sa_n_a = n_a} in
+  // start a new session wit this new state
+  let* sess_id = start_new_session bob ack_state in
+
+  // return the ID of the new session and the timestamp of the message
   return (Some (sess_id, ack_ts))
 
 
+/// Alice receives the reply from Bob:
+/// * read the message (n_a) from the trace
+/// * check if Alice previously sent n_a in some session
+/// * store completion of this session in a new state
+/// Returns the ID of the session that is marked as completed.
+/// The step fails, if
+/// * the message is not of the right type, i.e., not a reply
+/// * there is no prior session related to n_a
+
 val receive_ack: principal -> timestamp -> traceful (option state_id)
 let receive_ack alice ack_ts =
+  // receive the message and translate to abstract message type
   let*? ack = recv_msg ack_ts in
   let*? ack = return (parse message ack) in
+  // check that the message is a reply
+  // (otherwise this step fails)
   guard_tr (Ack? ack);*?
+
+  // read the data (n_a) from the message
   let Ack ack = ack in
+  let n_a = ack.a_n_a in
 
+  // check if alice has a previous session where
+  // * she startet a run
+  // * with the nonce n_a (the one received from Bob)
+  // (the step fails, if no such session exists)
   let*? (st, sid) = lookup_state #state alice
-    (fun st -> SentPing? st && (SentPing?.ping st).sp_n_a = ack.a_n_a)
-    in
+    (fun st -> 
+          SentPing? st // st is a state of type SentPing 
+      && (SentPing?.ping st).sp_n_a = n_a // the nonce stored in st is n_a
+    ) in
   guard_tr(SentPing? st);*?
-  let SentPing ping = st in
+  // access the name of Bob in the stored state
+  let bob = (SentPing?.ping st).sp_bob in
 
-  set_state alice sid (ReceivedAck {ra_bob=ping.sp_bob; ra_n_a = ack.a_n_a});*
+  // mark this session as completed by
+  // setting a new state
+  set_state alice sid (ReceivedAck {ra_bob = bob; ra_n_a = n_a});*
 
+  // return the ID of the completed session
   return (Some sid)
