examples/TwoMessageP/DY.TwoMessage.Run.Printing.fst
@@ -5,19 +5,23 @@ open DY.Lib
 open Comparse
 open DY.TwoMessage.Protocol
 
+/// Helper functions for trace printing.
+/// Here we define how our abstract message and state types
+/// should be printed.
+
 val message_to_string: bytes -> option string
 let message_to_string b =
   match? parse message b with
-  | Ping p -> Some (Printf.sprintf "Ping [prin = (%s), n_a = (%s)]" (p.p_alice) (bytes_to_string p.p_n_a))
+  | Ping p -> Some (Printf.sprintf "Ping [name = (%s), n_a = (%s)]" (p.p_alice) (bytes_to_string p.p_n_a))
   | Ack a -> Some (Printf.sprintf "Ping [n_a = (%s)]" (bytes_to_string a.a_n_a))
 
 
 val state_to_string: bytes -> option string
 let state_to_string b =
   match? parse state b with
-  | SentPing p -> Some (Printf.sprintf "SentPing [prin = (%s), n_a = (%s)]" p.sp_bob (bytes_to_string p.sp_n_a))
-  | SentAck a -> Some (Printf.sprintf "SentAck [prin = (%s), n_a = (%s)]" a.sa_alice (bytes_to_string a.sa_n_a))
-  | ReceivedAck r -> Some (Printf.sprintf "ReceivedAck [prin = (%s), n_a = (%s)]" r.ra_bob (bytes_to_string r.ra_n_a))
+  | SentPing p -> Some (Printf.sprintf "SentPing [to = (%s), n_a = (%s)]" p.sp_bob (bytes_to_string p.sp_n_a))
+  | SentAck a -> Some (Printf.sprintf "SentAck [to = (%s), n_a = (%s)]" a.sa_alice (bytes_to_string a.sa_n_a))
+  | ReceivedAck r -> Some (Printf.sprintf "ReceivedAck [from = (%s), n_a = (%s)]" r.ra_bob (bytes_to_string r.ra_n_a))
 
 
 
