examples/TwoMessageP/DY.TwoMessage.Run.fst
@@ -6,21 +6,31 @@ open DY.Lib
 open DY.TwoMessage.Run.Printing
 open DY.TwoMessage.Protocol
 
+/// Here, we print the trace after a successful run of the Two Message protocol.
+
 let run () : traceful (option unit ) =
   let _ = IO.debug_print_string "************* Trace *************\n" in
-  
-  let alice = "alice" in
-  let bob = "bob" in
 
+  // define the names of the two participants
+  let alice = "Alice" in
+  let bob = "Bob" in
+
+  // the actual protocol run
   let* (alice_sid, ping_ts) = send_ping alice bob in
-  let*? (bob_sid, ack_ts) = receive_ping_and_send_ack___ bob ping_ts in
+  // we pass the timestamp of Alice's ping to the receive function of Bob
+  let*? (bob_sid, ack_ts) = receive_ping_and_send_ack bob ping_ts in
+  // we pass the timestamp of Bob's response to the receive function of Alice
   let*? _ = receive_ack alice ack_ts in
 
+  // this part prints the resulting trace
   let* tr = get_trace in
   let _ = IO.debug_print_string (
       trace_to_string get_trace_to_string_printers tr
     ) in
 
   return (Some ())
-  
+
+
+/// Call `run` when the module loads
+
 let _ = run () Nil
